Refactor [sum] example, add comments

doc/tutorial/sum.v
@@ -1,4 +1,4 @@
-rom Coq Require Import String List ZArith.
+From Coq Require Import String List ZArith.
 From compcert Require Import Coqlib Integers Floats AST Ctypes Cop Clight Clightdefs.
 From compcert Require Import Maps Values ClightBigstep Events.
 
@@ -6,50 +6,78 @@ Require Import Clight.sum.
 
 Local Open Scope Z_scope.
 
+(* statement to be verified extracted from clightgen output *)
 Definition sum_statement := f_sum.(fn_body).
 
-Definition sum_fspec (s1 s2 : Z) := s1 + s2.
 
-Theorem f_sum_correct (ge : genv) (e : env) (m : Memory.Mem.mem) :
-  forall (ste : temp_env) (s1 s2 : Z),
-    ste ! _s1 = Some (Vint (Int.repr s1)) ->
-    ste ! _s2 = Some (Vint (Int.repr s2)) ->
-    Int.min_signed <= s1 <= Int.max_signed ->
-    Int.min_signed <= s2 <= Int.max_signed ->
-    exists (t : trace) (rte : temp_env),
-      exec_stmt ge e ste m sum_statement t rte m
-        (Out_return (Some ((Vint (Int.repr (sum_fspec s1 s2)), tint)))).
-Proof.
-  intros.
-  repeat eexists.
-  repeat econstructor.
-  - eassumption.
-  - eassumption.
-  - cbn.
-    unfold sem_binarith; simpl.
-    repeat rewrite cast_val_casted by (econstructor; auto).
-    repeat rewrite Int.add_signed.
-    repeat rewrite Int.signed_repr.
-    reflexivity.
-    assumption.
-    assumption.
-Qed.
+(** Specification using CompCert Int **)
+Section Int_spec.
+  
+  (* function specification of correctness *)
+  Definition sum_fspec_int (s1 s2 : int) := Int.add s1 s2.
+  
+  (* 
+   * if the starting temporary environment [ste] has values [s1] and [s2]
+   * assigned to identifiers "s1" and "s2", then there exist
+   * resulting trace [t] and resulting environment [rte], such that
+   * execution of [sum_statement] on [ste] results in a return with the correct value
+   *)
+  Theorem f_sum_correct_int (ge : genv) (e : env) (m : Memory.Mem.mem) :
+    forall (ste : temp_env) (s1 s2 : int),
+      ste ! _s1 = Some (Vint s1) ->
+      ste ! _s2 = Some (Vint s2) ->
 
-Definition sum_fspec_int (s1 s2 : int) := Int.add s1 s2.
+      exists (t : trace) (rte : temp_env),
+        exec_stmt ge e ste m sum_statement t rte m
+          (Out_return (Some (Vint (sum_fspec_int s1 s2), tint))).
+  Proof.
+    intros.
+    repeat eexists.
+    repeat econstructor.
+    - eassumption.
+    - eassumption.
+    - unfold sum_fspec_int.
+      constructor.
+  Qed.
 
-Theorem f_sum_correct_int (ge : genv) (e : env) (m : Memory.Mem.mem) :
-  forall (ste : temp_env) (s1 s2 : int),
-    ste ! _s1 = Some (Vint s1) ->
-    ste ! _s2 = Some (Vint s2) ->
-    exists (t : trace) (rte : temp_env),
-      exec_stmt ge e ste m sum_statement t rte m
-        (Out_return (Some (Vint (sum_fspec_int s1 s2), tint))).
-Proof.
-  intros.
-  repeat eexists.
-  repeat econstructor.
-  - eassumption.
-  - eassumption.
-  - unfold sum_fspec_int.
-    econstructor.
-Qed.
+End Int_spec.
+
+
+(** specification using Coq Z **)
+Section Z_spec.
+
+  (* specification now using Z instead of int *)
+  Definition sum_fspec_Z (s1 s2 : Z) := s1 + s2.
+  
+  (*
+   * the theorem is very similar, only with boundaries on Z values
+   * set (so that they fit int)
+   *)
+  Theorem f_sum_correct_Z (ge : genv) (e : env) (m : Memory.Mem.mem) :
+    forall (ste : temp_env) (s1 s2 : Z),
+      ste ! _s1 = Some (Vint (Int.repr s1)) ->
+      ste ! _s2 = Some (Vint (Int.repr s2)) ->
+
+      Int.min_signed <= s1 <= Int.max_signed ->
+      Int.min_signed <= s2 <= Int.max_signed ->
+
+      exists (t : trace) (rte : temp_env),
+        exec_stmt ge e ste m sum_statement t rte m
+          (Out_return (Some ((Vint (Int.repr (sum_fspec_Z s1 s2)), tint)))).
+  Proof.
+    intros.
+    repeat eexists.
+    repeat econstructor.
+    - eassumption.
+    - eassumption.
+    - cbn.
+      unfold sem_binarith; simpl.
+      repeat rewrite cast_val_casted by (econstructor; auto).
+      repeat rewrite Int.add_signed.
+      repeat rewrite Int.signed_repr.
+      reflexivity.
+      assumption.
+      assumption.
+  Qed.
+
+End Z_spec.
